src/PlutusIR/Semantics/TypeSafety/SubstitutionPreservesTyping/SubstituteTCA.v
@@ -2,7 +2,7 @@ Require Import PlutusCert.PlutusIR.
 Require Import PlutusCert.Util.List.
 From PlutusCert Require Import Kinding.Kinding Static.TypeSubstitution.
 
-
+Require Import Coq.Strings.String.
 
 (* See alpha_typing.v for a proof of this for STLC. This proof will be analogous*)
 Theorem substituteTCA_preserves_kinding : forall T Delta X K U L,
@@ -10,11 +10,11 @@ Theorem substituteTCA_preserves_kinding : forall T Delta X K U L,
     Delta |-* U : L ->
     Delta |-* (substituteTCA X U T) : K.
 Proof with eauto with typing.
-  (* induction T.
+  induction T.
   all: intros Delta X K U L Hkind__T HHkind__U.
   all: autorewrite with substituteTCA.
   all: simpl.
-  all: inversion Hkind__T; subst...
+  all: inversion Hkind__T; subst.
   - (* Ty_Var *)
     rename t into Y.
     destruct (X =? Y)%string eqn:Heqb.
@@ -25,11 +25,15 @@ Proof with eauto with typing.
       congruence.
     + (* X <> Y *)
       apply eqb_neq in Heqb as Hneq.
-      rewrite lookup_neq in H1...
+      rewrite lookup_neq in H1.
+      constructor. auto.
+      auto.
   - (* Ty_Forall *)
     admit.
+  - (* TY_IFIX*)
+    admit.
   - (* Ty_lam*)
-  admit. *)
+  admit.
 
     
 (* ADMIT: I had no time to finish this. Requires proofs about renamings. *)
